Insert switcher's invariant in FTLR

theories/examples/switcher/switcher_preamble.v
@@ -1,8 +1,9 @@
 From iris.algebra Require Import frac excl_auth.
 From iris.proofmode Require Import proofmode.
 From cap_machine Require Import logrel addr_reg_sample rules proofmode.
-From cap_machine Require Import multiple_updates region_invariants_revocation region_invariants_allocation.
-From cap_machine Require Import switcher.
+From cap_machine Require Import multiple_updates region_invariants_revocation.
+(* region_invariants_allocation. *)
+From cap_machine Require Export switcher.
 
 Section Switcher_preamble.
   Context
@@ -12,12 +13,14 @@ Section Switcher_preamble.
     {stsg : STSG Addr region_type Σ} {heapg : heapGS Σ}
     {tframeg : TFRAMEG Σ}
     {nainv: logrel_na_invs Σ}
-    `{MP: MachineParameters}.
+    `{MP: MachineParameters}
+    {swlayout : switcherLayout}
+  .
 
   Notation STS := (leibnizO (STS_states * STS_rels)).
   Notation STS_STD := (leibnizO (STS_std_states Addr region_type)).
-  Notation TFRAME := (leibnizO nat).
-  Notation WORLD := ( prodO (prodO STS_STD STS) TFRAME) .
+  Notation WORLD := (prodO STS_STD STS).
+  Notation STK := (leibnizO (list (Word * Word))).
   Implicit Types W : WORLD.
   Implicit Types C : CmptName.
 
@@ -41,18 +44,19 @@ Section Switcher_preamble.
           (⌜r ∉ (dom_arg_rmap ∪ {[PC; cra; cgp; csp]})⌝ →  ⌜reg !! r = Some (WInt 0)⌝)))%I.
   Solve All Obligations with solve_proper.
 
-  Program Definition execute_entry_point (wpcc wcgp : Word) (regs : Reg) : (WORLD -n> (leibnizO CmptName) -n> iPropO Σ) :=
+  Program Definition execute_entry_point (wpcc wcgp : Word) (regs : Reg) (cstk : STK) : (WORLD -n> (leibnizO CmptName) -n> iPropO Σ) :=
     (λne (W : WORLD) (C : CmptName),
        ( (execute_entry_point_register wpcc wcgp W C regs)
          ∗ registers_pointsto regs
          ∗ region W C
          ∗ sts_full_world W C
-         ∗ tframe_frag (frm W)
+         ∗ tframe_frag cstk
          ∗ na_own logrel_nais ⊤
            -∗ interp_conf W C)
     )%I.
   Solve All Obligations with solve_proper.
 
+  (* TODO unclear if it's still the right definition *)
   Program Definition ot_switcher_prop :
     (WORLD -n> (leibnizO CmptName) -n> (leibnizO Word) -n> iPropO Σ):=
     λne (W : WORLD) (C : CmptName) (w : Word),
@@ -68,10 +72,11 @@ Section Switcher_preamble.
            ∗ inv (export_table_PCCN C) ( b_tbl ↦ₐ WCap RX Global bpcc epcc bpcc)
            ∗ inv (export_table_CGPN C) ( (b_tbl ^+ 1)%a ↦ₐ WCap RW Global bcgp ecgp bcgp)
            ∗ inv (export_table_entryN C a_tbl) ( a_tbl ↦ₐ WInt (encode_entry_point nargs off))
-           ∗ □ ( ∀ W' regs, ⌜related_sts_priv_world W W'⌝ →
+           ∗ □ ( ∀ cstk W' regs, ⌜related_sts_priv_world W W'⌝ →
                    ▷ (execute_entry_point
                             (WCap RX Global bpcc epcc (bpcc ^+ off)%a)
                             (WCap RW Global bcgp ecgp bcgp)
+                            cstk
                             regs W' C))
       )%I.
   Solve All Obligations with solve_proper.
@@ -83,133 +88,133 @@ Section Switcher_preamble.
     persistent_cond ot_switcher_prop.
   Proof. intros [ [] ] ; cbn ; apply _. Qed.
 
-  Lemma mono_priv_ot_switcher (C : CmptName) (w : Word) :
-    ⊢ future_priv_mono C ot_switcher_propC w.
-  Proof.
-    iIntros (W W' Hrelated_W_W').
-    iModIntro.
-    iIntros "Hot_switcher".
-    iEval (cbn) in "Hot_switcher".
-    iEval (cbn).
-    iDestruct "Hot_switcher" as
-      (g_tbl b_tbl e_tbl a_tbl bpcc epcc bcgp ecgp nargs off ->
-       Hatbl Hbtbl Hbtbl1 Hnargs) "(Hinvpcc & Hinvcgp & Hinventry & #Hcont)".
-    iFrame "Hinvpcc Hinvcgp Hinventry".
-    iExists _,_.
-    repeat (iSplit ; first done).
-    iModIntro.
-    iIntros (W'' regs Hrelated_W'_W'').
-    iSpecialize ("Hcont" $! W'' regs).
-    iApply "Hcont".
-    iPureIntro.
-    by eapply related_sts_priv_trans_world.
-  Qed.
+  (* Lemma mono_priv_ot_switcher (C : CmptName) (w : Word) : *)
+  (*   ⊢ future_priv_mono C ot_switcher_propC w. *)
+  (* Proof. *)
+  (*   iIntros (W W' Hrelated_W_W'). *)
+  (*   iModIntro. *)
+  (*   iIntros "Hot_switcher". *)
+  (*   iEval (cbn) in "Hot_switcher". *)
+  (*   iEval (cbn). *)
+  (*   iDestruct "Hot_switcher" as *)
+  (*     (g_tbl b_tbl e_tbl a_tbl bpcc epcc bcgp ecgp nargs off -> *)
+  (*      Hatbl Hbtbl Hbtbl1 Hnargs) "(Hinvpcc & Hinvcgp & Hinventry & #Hcont)". *)
+  (*   iFrame "Hinvpcc Hinvcgp Hinventry". *)
+  (*   iExists _,_. *)
+  (*   repeat (iSplit ; first done). *)
+  (*   iModIntro. *)
+  (*   iIntros (W'' regs Hrelated_W'_W''). *)
+  (*   iSpecialize ("Hcont" $! W'' regs). *)
+  (*   iApply "Hcont". *)
+  (*   iPureIntro. *)
+  (*   by eapply related_sts_priv_trans_world. *)
+  (* Qed. *)
 
-  (** Custom invariant used by the switcher to store the frame  *)
-   Definition frame_inv (C : CmptName) (i : positive) (P : iProp Σ) :=
-     (∃ x:bool, sts_state_loc C i x ∗ if x then P else emp)%I.
-   Definition frame_rel_pub := λ (a b : bool), False.
-   Definition frame_rel_priv := λ (a b : bool), True.
-   Definition frame_W (W : WORLD) : WORLD :=
-     let ι := fresh_cus_name W in
-      <l[ ι := true , ( frame_rel_pub, (frame_rel_pub, frame_rel_priv)) ]l> W.
+  (* (** Custom invariant used by the switcher to store the frame  *) *)
+  (*  Definition frame_inv (C : CmptName) (i : positive) (P : iProp Σ) := *)
+  (*    (∃ x:bool, sts_state_loc C i x ∗ if x then P else emp)%I. *)
+  (*  Definition frame_rel_pub := λ (a b : bool), False. *)
+  (*  Definition frame_rel_priv := λ (a b : bool), True. *)
+  (*  Definition frame_W (W : WORLD) : WORLD := *)
+  (*    let ι := fresh_cus_name W in *)
+  (*     <l[ ι := true , ( frame_rel_pub, (frame_rel_pub, frame_rel_priv)) ]l> W. *)
 
-   Lemma frame_W_related_sts_pub_world (W : WORLD) : related_sts_pub_world W (frame_W W).
-   Proof.
-     rewrite /frame_W.
-     destruct W as [ [Wstd [fs fr] ] Wfrm ] .
-     assert (fresh (dom fs ∪ dom fr) ∉ (dom fs ∪ dom fr)) as Hfresh by apply is_fresh.
-     apply related_sts_pub_world_fresh_loc; set_solver.
-   Qed.
+  (*  Lemma frame_W_related_sts_pub_world (W : WORLD) : related_sts_pub_world W (frame_W W). *)
+  (*  Proof. *)
+  (*    rewrite /frame_W. *)
+  (*    destruct W as [ [Wstd [fs fr] ] Wfrm ] . *)
+  (*    assert (fresh (dom fs ∪ dom fr) ∉ (dom fs ∪ dom fr)) as Hfresh by apply is_fresh. *)
+  (*    apply related_sts_pub_world_fresh_loc; set_solver. *)
+  (*  Qed. *)
 
-   Set Nested Proofs Allowed.
+  (*  Set Nested Proofs Allowed. *)
 
-  Lemma frame_W_lookup_std (W : WORLD) (a : Addr) :
-    std (frame_W W) !! a = (std W) !!a.
-  Proof.
-    rewrite /frame_W.
-    by cbn.
-  Qed.
+  (* Lemma frame_W_lookup_std (W : WORLD) (a : Addr) : *)
+  (*   std (frame_W W) !! a = (std W) !!a. *)
+  (* Proof. *)
+  (*   rewrite /frame_W. *)
+  (*   by cbn. *)
+  (* Qed. *)
 
-  Lemma frame_W_lookup_loc (W : WORLD) (ι : positive) :
-    ι ≠ fresh_cus_name W ->
-    loc (frame_W W) !! ι = (loc W) !! ι.
-  Proof.
-    intros Hι.
-    rewrite /frame_W /= lookup_insert_ne //.
-  Qed.
-  Lemma frame_W_lookup_rel (W : WORLD) (ι : positive) :
-    ι ≠ fresh_cus_name W ->
-    wrel (frame_W W) !! ι = (wrel W) !! ι.
-  Proof.
-    intros Hι.
-    rewrite /frame_W /= lookup_insert_ne //.
-  Qed.
-  Lemma frame_W_lookup_frm (W : WORLD) : frm (frame_W W) = (frm W).
-  Proof. by cbn. Qed.
+  (* Lemma frame_W_lookup_loc (W : WORLD) (ι : positive) : *)
+  (*   ι ≠ fresh_cus_name W -> *)
+  (*   loc (frame_W W) !! ι = (loc W) !! ι. *)
+  (* Proof. *)
+  (*   intros Hι. *)
+  (*   rewrite /frame_W /= lookup_insert_ne //. *)
+  (* Qed. *)
+  (* Lemma frame_W_lookup_rel (W : WORLD) (ι : positive) : *)
+  (*   ι ≠ fresh_cus_name W -> *)
+  (*   wrel (frame_W W) !! ι = (wrel W) !! ι. *)
+  (* Proof. *)
+  (*   intros Hι. *)
+  (*   rewrite /frame_W /= lookup_insert_ne //. *)
+  (* Qed. *)
+  (* Lemma frame_W_lookup_frm (W : WORLD) : frm (frame_W W) = (frm W). *)
+  (* Proof. by cbn. Qed. *)
 
-  Lemma ι0_in_Wloc_helper (W0 : WORLD) (ι0 : positive) (callee_stk_frm_addr : list Addr) :
-    ι0 ∈ (dom (loc (std_update_multiple
-                       (<l[ι0:=false]l>(revoke W0))
-                       callee_stk_frm_addr Temporary))).
-  Proof.
-    rewrite std_update_multiple_loc_sta dom_insert_L; set_solver.
-  Qed.
+  (* Lemma ι0_in_Wloc_helper (W0 : WORLD) (ι0 : positive) (callee_stk_frm_addr : list Addr) : *)
+  (*   ι0 ∈ (dom (loc (std_update_multiple *)
+  (*                      (<l[ι0:=false]l>(revoke W0)) *)
+  (*                      callee_stk_frm_addr Temporary))). *)
+  (* Proof. *)
+  (*   rewrite std_update_multiple_loc_sta dom_insert_L; set_solver. *)
+  (* Qed. *)
 
-  Lemma ι0_isnot_fresh (W0 : WORLD) (ι0 : positive) (callee_stk_frm_addr : list Addr) :
-    ι0 ≠ fresh_cus_name (std_update_multiple
-                           (<l[ι0:=false]l>(revoke W0))
-                           callee_stk_frm_addr Temporary).
-  Proof.
-    apply fresh_name_notin. left.
-    apply ι0_in_Wloc_helper.
-  Qed.
-
-
-  (** Evolution of the world in the switcher *)
-  Definition switcher_world_pre_frame (W_init : WORLD) (callee_stk_frm_addr : list Addr) :=
-    (std_update_multiple (<d[ frm W_init + 1]d>(revoke W_init)) callee_stk_frm_addr Temporary).
-
-  Definition switcher_world_upon_jmp (W_init : WORLD)
-    (a_local_args callee_stk_frm_addr : list Addr) :=
-    std_update_multiple
-      (frame_W (switcher_world_pre_frame W_init callee_stk_frm_addr))
-      a_local_args Temporary.
-
-  Lemma related_sts_priv_world_switcher_pre_frame
-    (W : WORLD) (callee_stk_frm_addr : list Addr) :
-    Forall (fun a => std W !! a = Some Revoked) callee_stk_frm_addr ->
-    related_sts_priv_world W (switcher_world_pre_frame W callee_stk_frm_addr).
-  Proof.
-    intros Ha_local_args.
-    rewrite /switcher_world_pre_frame.
-    eapply related_sts_priv_trans_world; cycle 1.
-    { apply related_sts_pub_priv_world.
-      apply related_sts_pub_update_multiple_temp.
-      eapply Forall_impl; eauto.
-      intros a Ha; cbn in *.
-      by apply revoke_lookup_Revoked.
-    }
-    eapply related_sts_priv_trans_world; cycle 1.
-    { apply sts.related_sts_priv_world_update_frm. }
-    apply revoke_related_sts_priv_world.
-  Qed.
+  (* Lemma ι0_isnot_fresh (W0 : WORLD) (ι0 : positive) (callee_stk_frm_addr : list Addr) : *)
+  (*   ι0 ≠ fresh_cus_name (std_update_multiple *)
+  (*                          (<l[ι0:=false]l>(revoke W0)) *)
+  (*                          callee_stk_frm_addr Temporary). *)
+  (* Proof. *)
+  (*   apply fresh_name_notin. left. *)
+  (*   apply ι0_in_Wloc_helper. *)
+  (* Qed. *)
 
 
-  Definition switcher_inv
-    (b_switcher e_switcher a_switcher_cc b_tstk e_tstk : Addr)
-    (ot_switcher : OType) : iProp Σ :=
-    ∃ (a_tstk : Addr) (d : nat) (tstk_next : list Word),
-     mtdc ↦ₛᵣ WCap RWL Local b_tstk e_tstk a_tstk
-     ∗ ⌜ SubBounds
-         b_switcher e_switcher
-         a_switcher_cc (a_switcher_cc ^+ length switcher_instrs)%a ⌝
+  (* (** Evolution of the world in the switcher *) *)
+  (* Definition switcher_world_pre_frame (W_init : WORLD) (callee_stk_frm_addr : list Addr) := *)
+  (*   (std_update_multiple (<d[ frm W_init + 1]d>(revoke W_init)) callee_stk_frm_addr Temporary). *)
+
+  (* Definition switcher_world_upon_jmp (W_init : WORLD) *)
+  (*   (a_local_args callee_stk_frm_addr : list Addr) := *)
+  (*   std_update_multiple *)
+  (*     (frame_W (switcher_world_pre_frame W_init callee_stk_frm_addr)) *)
+  (*     a_local_args Temporary. *)
+
+  (* Lemma related_sts_priv_world_switcher_pre_frame *)
+  (*   (W : WORLD) (callee_stk_frm_addr : list Addr) : *)
+  (*   Forall (fun a => std W !! a = Some Revoked) callee_stk_frm_addr -> *)
+  (*   related_sts_priv_world W (switcher_world_pre_frame W callee_stk_frm_addr). *)
+  (* Proof. *)
+  (*   intros Ha_local_args. *)
+  (*   rewrite /switcher_world_pre_frame. *)
+  (*   eapply related_sts_priv_trans_world; cycle 1. *)
+  (*   { apply related_sts_pub_priv_world. *)
+  (*     apply related_sts_pub_update_multiple_temp. *)
+  (*     eapply Forall_impl; eauto. *)
+  (*     intros a Ha; cbn in *. *)
+  (*     by apply revoke_lookup_Revoked. *)
+  (*   } *)
+  (*   eapply related_sts_priv_trans_world; cycle 1. *)
+  (*   { apply sts.related_sts_priv_world_update_frm. } *)
+  (*   apply revoke_related_sts_priv_world. *)
+  (* Qed. *)
+
+
+  Definition switcher_inv : iProp Σ :=
+    ∃ (a_tstk : Addr) (cstk : STK) (tstk_next : list Word),
+     mtdc ↦ₛᵣ WCap RWL Local b_trusted_stack e_trusted_stack a_tstk
+     (* ∗ ⌜ SubBounds *)
+     (*     b_switcher e_switcher *)
+     (*     a_switcher_call (a_switcher_call ^+ length switcher_instrs)%a ⌝ *)
      ∗ ⌜ (ot_switcher < (ot_switcher ^+1) )%ot ⌝
-     ∗ codefrag a_switcher_cc switcher_instrs
+     ∗ codefrag a_switcher_call switcher_instrs
      ∗ b_switcher ↦ₐ WSealRange (true,true) Global ot_switcher (ot_switcher^+1)%ot ot_switcher
-     ∗ [[ (a_tstk ^+1)%a, e_tstk ]] ↦ₐ [[ tstk_next ]]
-     ∗ ⌜ (b_tstk <= a_tstk)%a ∧ (a_tstk <= e_tstk)%a ⌝
-     ∗ tframe_full d ∗ ⌜ (b_tstk + d)%a = Some a_tstk  ⌝
+     ∗ [[ (a_tstk ^+1)%a, e_trusted_stack ]] ↦ₐ [[ tstk_next ]]
+     ∗ ⌜ (b_trusted_stack <= a_tstk)%a ∧ (a_tstk <= e_trusted_stack)%a ⌝
+     ∗ tframe_full cstk
+     ∗ ⌜ (b_trusted_stack + length cstk)%a = Some a_tstk  ⌝
+     ∗ True (* TODO link the topmost frame of cstk to the state *)
      ∗ seal_pred ot_switcher ot_switcher_propC.
 
 
